Try a much simpler version based on today's discussion with Joe.

CrSemantics.v
@@ -4,7 +4,6 @@ Require Import List.
 Import ListNotations.
 Require Import Strings.String.
 From MyProject Require Export CrIdentifiers.
-From MyProject Require Export Map.
 
 (* TODO: fill out eval_transformer body at the end,
    right now, we are just specifying it as a function that
@@ -28,9 +27,17 @@ Parameter eval_seq_rule : MatchActionRule -> Valuation -> Valuation.
    meaning header ops within an action are evaluated in parallel *)
 Parameter eval_par_rule : MatchActionRule -> Valuation -> Valuation.
 
+(* Expression version of a header operation, meaning side-effect-free and stateless *)
+Definition eval_hdr_op_expr (op : HdrOp) (v : Valuation) : uint8 :=
+    match op with
+    | StatefulOp f arg1 arg2 target => apply_bin_op f (function_argument_to_uint8 arg1 v) (function_argument_to_uint8 arg2 v)
+    | StatelessOp f arg1 arg2 target => apply_bin_op f (function_argument_to_uint8 arg1 v) (function_argument_to_uint8 arg2 v)
+    end.
+
 (* Function to evaluate a header operation,
    meaning we apply the operation to a previous valuation to get a new one *)
-Definition eval_hdr_op (op : HdrOp) (input_valuation : Valuation) : Valuation :=
+(*
+   Definition eval_hdr_op (op : HdrOp) (input_valuation : Valuation) : Valuation :=
     match op with
     | StatefulOp f arg1 arg2 target =>
         let new_state :=
@@ -48,3 +55,4 @@ Definition eval_hdr_op (op : HdrOp) (input_valuation : Valuation) : Valuation :=
                state_var_map := state_var_map input_valuation |}  (* Leave this unchanged *)
     end.
 (*TODO: Maybe figure out a way to unify parsing and header manipulation into seq and par transformers respectively. *)
+*)
