SmtExpr.v
@@ -3,6 +3,8 @@
 From MyProject Require Import CrIdentifiers.
 From Coq.Strings Require Import String.
 
+Definition SmtValuation := string -> uint8.
+
 (* Basic starting point of Smt expressions, just have 8 bit ands, ors, and nots.
    Can express everything a sat solver cares about by just setting 7 bits to zero.
    so seems complete in some sense.*)
@@ -30,13 +32,12 @@ Definition SmtResult_eqb (a b : SmtResult) : bool :=
 Parameter smt_query_engine : SmtExpr -> SmtResult.
 
 (* Provide semantics for the SmtExpr above using the uint8 functions from Integer.v *)
-Fixpoint eval_smt_expr (e : SmtExpr) (v : fmap string uint8) : uint8 :=
+Fixpoint eval_smt_expr (e : SmtExpr) (v : SmtValuation) : uint8 :=
     match e with
     | SmtConst value => value
-    | SmtVar name => match lookup v name with
-                     | Some value => value
-                     | None => zero (* Default to zero if variable not found *)
-                     end
+    | SmtVar name => v name
+    (* Note: we assume that the valuation v is well-formed,
+       i.e., it contains all the variables that appear in the expression *)
     | SmtBitAdd e1 e2 => add (eval_smt_expr e1 v) (eval_smt_expr e2 v)
     | SmtBitAnd e1 e2 => and (eval_smt_expr e1 v) (eval_smt_expr e2 v)
     | SmtBitOr e1 e2 => or (eval_smt_expr e1 v) (eval_smt_expr e2 v)
